\documentclass{article}
\usepackage{amsfonts}
\usepackage{amsmath}
\usepackage{hyperref}
\usepackage[left=2cm,right=2cm,top=2cm,bottom=2cm]{geometry}
%\newenvironment{amatrix}[1]{%
%  \left(\begin{array}{@{}*{#1}{c}|c@{}}
%}{%
%  \end{array}\right)
%}

\author{Mark Vijfvinkel \& Aram Verstegen \\ 0863002(s134674), s4092368 \\ Radboud University}
\title{Cryptography 1, Homework 4}

\begin{document}
\maketitle
\date

\section{}
\begin{equation}
\begin{aligned}
 a &= (649,1,0) \\
 b &= (155,0,1) \\
c &= a - 4 \cdot b &= (29,1,-4), \mbox{where (c, coefficient of a, coefficient of b)} \\
a &= (155,0,1) \\
b &= (29,1,-4) \\
c &= a - 5 \cdot b &= (10,-5,21) \\
a &= (29,1,-4) \\
b &= (10,-5,21) \\
c &= a - 2 \cdot b &= (9,11,-46) \\
a &= (10,-5,21) \\
b &= (9,11,-46) \\
c &= a-b &= (1,-16,67) \\
d,u,v &= 1,-16,67
\end{aligned}
\end{equation}

\section{}
\begin{equation}
\begin{aligned}
a &= (6891,1,0) \\
b &= (5007,0,1) \\
c &= a-b &= (1884,1,-1) \\
a &= (5007,0,1) \\
b &= (1884,1,-1) \\
c &= a-2b &= (1239,-2,3) \\
a &= (1884,1,-1) \\
b &= (1239,-2,3) \\
c &= a-b &= (645,3,-4) \\
a &= (1239,-2,3) \\
b &= (645,3,-4) \\
c &= a-b &= (594,-5,7) \\
a &= (645,3,-4) \\
b &= (594,-5,7) \\
c &= a-b &= (51,8,-11) \\
a &= (594,-5,7) \\
b &= (51,8,-11) \\
c &= a-11b &= (33,-93,128) \\
a &= (51,8,-11) \\
b &= (33,-93,128) \\
c &= a-b &= (18,101,-139) \\
a &= (33,-93,128) \\
b &= (18,101,-139) \\
c &= a-b &= (15,-194,267) \\
a &= (18,101,-139) \\
b &= (15,-194,267) \\
c &= a-b &= (3,295,-406) \\
a &= (15,-194,267) \\
b &= (3,295,-406) \\
d,u,v&=3,295,-406
\end{aligned}
\end{equation}

\section{}
\begin{equation}
\begin{aligned}
a &= (x^5 + 3x^3 + x^2 + 2x + 1, 1, 0) \\
b &= (x^4 - 5x^3 - 5x^2 - 5x - 6, 0, 1) \\
c &= (a-(x+5)b) \\
  &= (33x^3+31x^2+33x+31, 1, -x-5) \\
a &= (x^4 - 5x^3 - 5x^2 - 5x - 6, 0, 1) \\
b &= (33x^3+31x^2+33x+31, 1, -x-5) \\
c &= a-(x/33 - 196/1089)b \\
  &= (-458/1089x^2 + 458/1089, -1/33x + 196/1089, 1/33x^2 - 31/1089x + 109/1089) \\
a &= (33x^3+31x^2+33x+31, 1, -x-5) \\
b &= (-458/1089x^2 + 458/1089, -1/33x + 196/1089, 1/33x^2 - 31/1089x + 109/1089) \\
c &= a-(-35937/458x - 33759/458)b \\
  &= (0, -1089/458x^2 + 5445/458x + 3267/229, 1089/458x^3 + 1089/229x + 1089/458)\\
a &= (-458/1089x^2 - 458/1089, -1/33x + 196/1089, 1/33x^2 - 31/1089x + 109/1089) \\
b &= (0, -1089/458x^2 + 5445/458x + 3267/229, 1089/458x^3 + 1089/229x + 1089/458) \\
d,u,v &= (x^2 +1, 33/458x - 98/229, -33/458x^2 + 31/458x - 109/458)
\end{aligned}
\end{equation}

\section{}
\begin{equation}
\begin{aligned}
a &= (x^{11} + x^9 + x^7 + x^4 + x^3 + x + 1, 1, 0) \\
b &= (x^8 + x^5 + x^4 + x^3 + x + 1, 0, 1) \\
c &= (a-(x^3 + x + 1)b) \\
  &= (x^3 + x^2 + x, 1, -x^3 - x - 1) \\
a &= (x^8 + x^5 + x^4 + x^3 + x + 1, 0, 1) \\
b &= (x^3 + x^2 + x, 1, -x^3 - x - 1) \\
c &= a-(x^5 + x^4 + x)b \\
  &= (x^2 + x + 1, x^5 + x^4 + x, x^8 + x^7 + x^6 + x^2 + x + 1) \\
a &= (x^3 + x^2 + x, 1, -x^3 - x - 1) \\
b &= (x^2 + x + 1, x^5 + x^4 + x, x^8 + x^7 + x^6 + x^2 + x + 1) \\
c &= a-xb \\
  &= (0, x^6 + x^5 + x^2 + 1, x^9 + x^8 + x^7 + x^2 + 1) \\
a &= (x^2 + x + 1, x^5 + x^4 + x, x^8 + x^7 + x^6 + x^2 + x + 1) \\
b &= (0, x^6 + x^5 + x^2 + 1, x^9 + x^8 + x^7 + x^2 + 1) \\
d,u,v &= (x^2 + x + 1, x^5 + x^4 + x, x^8 + x^7 + x^6 + x^2 + x + 1)
\end{aligned}
\end{equation}

\end{document}
